sorry-free

src/Init/Data/Range/Polymorphic/BitVec.lean
@@ -11,11 +11,11 @@ public import Init.Data.Order.Lemmas
 public import Init.Data.UInt
 import Init.Omega
 
-public section
-
 open Std Std.PRange
 
 namespace BitVec
+
+public section
 
 variable {n : Nat}
 
@@ -81,12 +81,11 @@ instance : LawfulUpwardEnumerableLE (BitVec n) where
       simp [BitVec.ofNatLT]
 
 instance : LawfulUpwardEnumerableLT (BitVec n) := inferInstance
-instance : LawfulUpwardEnumerableLT (BitVec n) := inferInstance
 
-instance : Rxc.HasSize (BitVec n) where
+instance instRxcHasSize : Rxc.HasSize (BitVec n) where
   size lo hi := hi.toNat + 1 - lo.toNat
 
-instance : Rxc.LawfulHasSize (BitVec n) where
+instance instRxcLawfulHasSize : Rxc.LawfulHasSize (BitVec n) where
   size_eq_zero_of_not_le bound x := by
     simp only [BitVec.not_le, Rxc.HasSize.size, BitVec.lt_def]
     omega
@@ -98,16 +97,16 @@ instance : Rxc.LawfulHasSize (BitVec n) where
     simp only [succ?_eq_some, Rxc.HasSize.size, BitVec.le_def]
     omega
 
-instance : Rxc.IsAlwaysFinite (BitVec n) := inferInstance
+instance instRxcIsAlwaysFinite : Rxc.IsAlwaysFinite (BitVec n) := inferInstance
 
-instance : Rxo.HasSize (BitVec n) := .ofClosed
-instance : Rxo.LawfulHasSize (BitVec n) := inferInstance
-instance : Rxo.IsAlwaysFinite (BitVec n) := inferInstance
+instance instRxoHasSize : Rxo.HasSize (BitVec n) := .ofClosed
+instance instRxoLawfulHasSize : Rxo.LawfulHasSize (BitVec n) := inferInstance
+instance instRxoIsAlwaysFinite : Rxo.IsAlwaysFinite (BitVec n) := inferInstance
 
-instance : Rxi.HasSize (BitVec n) where
+instance instRxiHasSize : Rxi.HasSize (BitVec n) where
   size lo := 2 ^ n - lo.toNat
 
-instance : Rxi.LawfulHasSize (BitVec n) where
+instance instRxiLawfulHasSize : Rxi.LawfulHasSize (BitVec n) where
   size_eq_one_of_succ?_eq_none x := by
     simp only [succ?_eq_none, Rxi.HasSize.size]
     omega
@@ -115,343 +114,7 @@ instance : Rxi.LawfulHasSize (BitVec n) where
     simp only [succ?_eq_some, Rxi.HasSize.size]
     omega
 
-instance : Rxi.IsAlwaysFinite (BitVec n) := inferInstance
+instance instRxiIsAlwaysFinite : Rxi.IsAlwaysFinite (BitVec n) := inferInstance
 
-namespace Signed
-
-def irredMin n : BitVec n := ↑(2 ^ (n - 1) : Nat)
-theorem irredMin_def : irredMin n = ↑(2 ^ (n - 1) : Nat) := (rfl)
-seal irredMin
-
-def irredMax n : BitVec n := ↑(2 ^ (n - 1) - 1 : Nat)
-theorem irredMax_def : irredMax n = ↑(2 ^ (n - 1) - 1 : Nat) := (rfl)
-seal irredMax
-
-@[expose]
-def rotate (x : BitVec n) : BitVec n := x + irredMin n
-
-theorem irredMax_eq_irredMin_add :
-    irredMax n = irredMin n + ↑(2 ^ n - 1 : Nat) := by
-  match n with
-  | 0 => simp [eq_nil (irredMax 0), eq_nil (irredMin 0)]
-  | n + 1 =>
-    simp only [irredMax_def, Nat.add_one_sub_one, natCast_eq_ofNat, irredMin_def, ← ofNat_add,
-      ← toNat_inj, toNat_ofNat, Nat.mod_eq_mod_iff]
-    exact ⟨1, 0, by omega⟩
-
-theorem irredMin_add_irredMin :
-    irredMin n + irredMin n = 0 := by
-  match n with
-  | 0 => simp [eq_nil (irredMin 0)]
-  | n + 1 =>
-    simp [irredMin_def, ← BitVec.ofNat_add, show 2 ^ n + 2 ^ n = 2 ^ (n + 1) by omega,
-      ← BitVec.toNat_inj]
-
-theorem rotate_neg_eq_irredMin_sub {x : BitVec n} :
-    rotate (-x) = irredMin n - x := by
-  simp only [rotate, irredMin_def, natCast_eq_ofNat]
-  rw [eq_sub_iff_add_eq, BitVec.add_comm, ← BitVec.add_assoc, BitVec.add_neg_eq_sub,
-    BitVec.sub_self, BitVec.zero_add]
-
-theorem rotate_eq_sub_irredMin {x : BitVec n} :
-    rotate x = x - irredMin n := by
-  simp [rotate, eq_sub_iff_add_eq, BitVec.add_assoc, irredMin_add_irredMin]
-
-theorem rotate_add {x y : BitVec n} :
-    rotate (x + y) = rotate x + y := by
-  simp [rotate, BitVec.add_assoc, BitVec.add_comm y]
-
-theorem rotate_sub {x y : BitVec n} :
-    rotate (x - y) = rotate x - y := by
-  simp [BitVec.sub_eq_add_neg, rotate_add]
-
-theorem rotate_irredMin :
-    rotate (irredMin n) = ↑(0 : Nat) := by
-  simp [rotate, irredMin_add_irredMin]
-
-theorem rotate_irredMax :
-    rotate (irredMax n) = ↑(2 ^ n - 1 : Nat) := by
-  simp [irredMax_eq_irredMin_add, rotate_add, rotate_irredMin]
-
-theorem rotate_rotate {x : BitVec n} :
-    rotate (rotate x) = x := by
-  match n with
-  | 0 => simp [eq_nil x, rotate, irredMin_def]
-  | n + 1 =>
-    simp only [rotate, BitVec.add_assoc]
-    simp [← BitVec.toNat_inj, ← Nat.two_mul, irredMin_def, show 2 * 2 ^ n = 2 ^ (n + 1) by omega]
-
-theorem rotate_map_eq_iff {x y : Option (BitVec n)} :
-    rotate <$> x = y ↔ x = rotate <$> y := by
-  suffices h : ∀ x y : Option (BitVec n), rotate <$> x = y → x = rotate <$> y by
-    exact ⟨h x y, fun h' => (h y x h'.symm).symm⟩
-  intro x y h
-  replace h := congrArg (rotate <$> ·) h
-  simpa [Function.comp_def, rotate_rotate] using h
-
-scoped instance instUpwardEnumerable : UpwardEnumerable (BitVec n) where
-  succ? x := rotate <$> UpwardEnumerable.succ? (rotate x)
-  succMany? n x := rotate <$> UpwardEnumerable.succMany? n (rotate x)
-
-theorem succ?_rotate {x : BitVec n} :
-    succ? (rotate x) = (haveI := BitVec.instUpwardEnumerable (n := n); rotate <$> succ? x) := by
-  simp [succ?, rotate_rotate]
-
-theorem succMany?_rotate {x : BitVec n} :
-    succMany? m (rotate x) =
-      (haveI := BitVec.instUpwardEnumerable (n := n); rotate <$> succMany? m x) := by
-  simp [succMany?, rotate_rotate]
-
-theorem sle_iff_rotate_le_rotate {x y : BitVec n} :
-    x.sle y ↔ rotate x ≤ rotate y := by
-  match n with
-  | 0 => simp [eq_nil x, eq_nil y]
-  | n + 1 =>
-    simp [BitVec.sle_iff_toInt_le, BitVec.toInt, Nat.pow_add, Nat.mul_comm _ 2, rotate, BitVec.le_def,
-      irredMin_def]
-    split <;> split
-    · simp only [Int.ofNat_le]
-      rw [Nat.mod_eq_of_lt (by omega), Nat.mod_eq_of_lt (by omega)]
-      omega
-    · have : (↑y.toNat : Int) - 2 * 2 ^ n < 0 := by
-        have := BitVec.toNat_lt_twoPow_of_le (x := y) (Nat.le_refl _)
-        simp [Nat.pow_add, Nat.mul_comm _ 2] at this
-        simp only [← Int.ofNat_lt, Int.natCast_mul, Int.cast_ofNat_Int, Int.natCast_pow] at this
-        omega
-      have : ¬ (↑x.toNat ≤ (↑y.toNat : Int) - 2 * 2 ^ n) := by
-        apply Int.not_le_of_gt
-        calc _ < 0 := this
-             _ ≤ _ := by omega
-      simp [this]
-      rw [Nat.mod_eq_mod_iff (x := y.toNat + 2 ^ n) (y := y.toNat - 2 ^ n) (z := 2 * 2 ^ n) |>.mpr]
-      rotate_left
-      · exact ⟨0, 1, by omega⟩
-      rw [Nat.mod_eq_of_lt (by omega), Nat.mod_eq_of_lt (by omega)]
-      omega
-    · have : (↑x.toNat : Int) - 2 * 2 ^ n ≤ ↑y.toNat := by
-        have : x.toNat < 2 * 2 ^ n := by omega
-        have : (↑x.toNat : Int) < 2 * 2 ^ n := by simpa [← Int.ofNat_lt] using this
-        omega
-      simp [this]
-      rw [Nat.mod_eq_mod_iff (x := x.toNat + 2 ^ n) (y := x.toNat - 2 ^ n) (z := 2 * 2 ^ n) |>.mpr]
-      rotate_left
-      · exact ⟨0, 1, by omega⟩
-      rw [Nat.mod_eq_of_lt (by omega), Nat.mod_eq_of_lt (by omega)]
-      omega
-    · simp
-      rw [Nat.mod_eq_mod_iff (x := x.toNat + 2 ^ n) (y := x.toNat - 2 ^ n) (z := 2 * 2 ^ n) |>.mpr ⟨0, 1, by omega⟩,
-        Nat.mod_eq_mod_iff (x := y.toNat + 2 ^ n) (y := y.toNat - 2 ^ n) (z := 2 * 2 ^ n) |>.mpr ⟨0, 1, by omega⟩,
-        Nat.mod_eq_of_lt (by omega), Nat.mod_eq_of_lt (by omega)]
-      omega
-
-theorem rotate_inj {x y : BitVec n} :
-    rotate x = rotate y ↔ x = y := by
-  apply Iff.intro
-  · intro h
-    simpa [rotate_rotate] using congrArg rotate h
-  · intro h
-    exact congrArg rotate h
-
-theorem rotate_eq_iff {x y : BitVec n} :
-    rotate x = y ↔ x = rotate y := by
-  rw [← rotate_rotate (x := y), rotate_inj, rotate_rotate]
-
-theorem toInt_eq_ofNat_toNat_rotate_sub' {x : BitVec n} (h : n > 0) :
-    x.toInt = (↑(rotate x).toNat : Int) - ↑(irredMin n).toNat := by
-  match n with
-  | 0 => omega
-  | n + 1 =>
-    simp [BitVec.toInt, rotate, irredMin_def]
-    rw [Int.emod_eq_of_lt (a := 2 ^ n)]; rotate_left
-    · exact Int.le_of_lt (Int.pow_pos (by omega))
-    · rw [Int.pow_add, Int.pow_succ, Int.pow_zero, Int.one_mul, Int.mul_comm, Int.two_mul]
-      exact Int.lt_add_of_pos_right _ (Int.pow_pos (by omega))
-    have : (2 : Int) ^ n > 0 := Int.pow_pos (by omega)
-    split <;> rename_i h
-    · rw [Nat.pow_add, Nat.pow_one, Nat.mul_comm _ 2, Nat.mul_lt_mul_left (by omega),
-        ← Int.ofNat_lt, Int.natCast_pow, Int.cast_ofNat_Int] at h
-      rw [Int.emod_eq_of_lt (by omega) (by omega)]
-      omega
-    · rw [Nat.pow_add, Nat.pow_one, Nat.mul_comm _ 2, Nat.mul_lt_mul_left (by omega),
-        ← Int.ofNat_lt, Int.natCast_pow, Int.cast_ofNat_Int] at h
-      simp [Int.pow_add, Int.mul_comm _ 2, Int.two_mul, ← Int.sub_sub]
-      rw [eq_comm, Int.emod_eq_iff (by omega)]
-      refine ⟨by omega, ?_, ?_⟩
-      · have := BitVec.toNat_lt_twoPow_of_le (x := x) (Nat.le_refl _)
-        rw [Int.ofNat_natAbs_of_nonneg (by omega)]
-        simp only [Nat.pow_add, Nat.pow_one, ← Int.ofNat_lt, Int.natCast_mul, Int.natCast_pow,
-          Int.cast_ofNat_Int] at this
-        omega
-      · conv => rhs; rw [← Int.sub_sub, Int.sub_sub (b := 2 ^ n), Int.add_comm, ← Int.sub_sub]
-        exact ⟨-1, by omega⟩
-
-theorem toInt_eq_ofNat_toNat_rotate_sub {x : BitVec n} (h : n > 0) :
-    x.toInt = (↑(rotate x).toNat : Int) - 2 ^ (n - 1) := by
-  match n with
-  | 0 => omega
-  | n + 1 =>
-    simp [BitVec.toInt, rotate, irredMin_def]
-    have : (2 : Int) ^ n > 0 := Int.pow_pos (by omega)
-    split <;> rename_i h
-    · rw [Nat.pow_add, Nat.pow_one, Nat.mul_comm _ 2, Nat.mul_lt_mul_left (by omega),
-        ← Int.ofNat_lt, Int.natCast_pow, Int.cast_ofNat_Int] at h
-      rw [Int.emod_eq_of_lt (by omega) (by omega)]
-      omega
-    · rw [Nat.pow_add, Nat.pow_one, Nat.mul_comm _ 2, Nat.mul_lt_mul_left (by omega),
-        ← Int.ofNat_lt, Int.natCast_pow, Int.cast_ofNat_Int] at h
-      simp [Int.pow_add, Int.mul_comm _ 2, Int.two_mul, ← Int.sub_sub]
-      rw [eq_comm, Int.emod_eq_iff (by omega)]
-      refine ⟨by omega, ?_, ?_⟩
-      · have := BitVec.toNat_lt_twoPow_of_le (x := x) (Nat.le_refl _)
-        rw [Int.ofNat_natAbs_of_nonneg (by omega)]
-        simp only [Nat.pow_add, Nat.pow_one, ← Int.ofNat_lt, Int.natCast_mul, Int.natCast_pow,
-          Int.cast_ofNat_Int] at this
-        omega
-      · conv => rhs; rw [← Int.sub_sub, Int.sub_sub (b := 2 ^ n), Int.add_comm, ← Int.sub_sub]
-        exact ⟨-1, by omega⟩
-
-theorem ofNat_eq_rotate_ofInt_sub {n k : Nat} :
-    BitVec.ofNat n k = rotate (BitVec.ofInt n (↑k - ↑(irredMin n).toNat)) := by
-  match n with
-  | 0 => simp only [eq_nil (BitVec.ofNat _ _), eq_nil (rotate _)]
-  | n + 1 =>
-    simp [irredMin]
-    rw [Int.emod_eq_of_lt]; rotate_left
-    · exact Int.le_of_lt (Int.pow_pos (by omega))
-    · exact Int.pow_lt_pow_of_lt (by omega) (by omega)
-    simp [← BitVec.toInt_inj, toInt_ofNat', rotate, Int.bmod_eq_bmod_iff_bmod_sub_eq_zero]
-    simp [Int.sub_eq_add_neg, Int.neg_add, ← Int.add_assoc]
-    simp [Int.add_neg_eq_sub, irredMin, toInt_ofNat']
-
-scoped instance instLE : LE (BitVec n) where
-  le x y := x.sle y
-
-scoped instance : DecidableLE (BitVec n) := fun x y => inferInstanceAs (Decidable <| x.sle y)
-
-scoped instance instLT : LT (BitVec n) where
-  lt x y := x.slt y
-
-scoped instance : DecidableLT (BitVec n) := fun x y => inferInstanceAs (Decidable <| x.slt y)
-
-scoped instance : LawfulOrderLT (BitVec n) where
-  lt_iff x y := by
-    simp only [LE.le, LT.lt]
-    simpa [BitVec.slt_iff_toInt_lt, BitVec.sle_iff_toInt_le] using Int.le_of_lt
-
-scoped instance : IsPartialOrder (BitVec n) where
-  le_refl x := by simp only [LE.le]; simp [BitVec.sle_iff_toInt_le]
-  le_trans := by
-    simp only [LE.le]
-    simpa [BitVec.sle_iff_toInt_le] using fun _ _ _ => Int.le_trans
-  le_antisymm := by
-    simp only [LE.le, ← BitVec.toInt_inj]
-    simpa [BitVec.sle_iff_toInt_le] using fun _ _ => Int.le_antisymm
-
-scoped instance : LawfulUpwardEnumerableLE (BitVec n) where
-  le_iff x y := by
-    rw [← rotate_rotate (x := x), ← rotate_rotate (x := y)]
-    generalize (rotate x) = x
-    generalize (rotate y) = y
-    simp only [LE.le]
-    rw [sle_iff_rotate_le_rotate]
-    letI := BitVec.instUpwardEnumerable (n := n)
-    letI := instLEBitVec (w := n)
-    simp [UpwardEnumerable.le_iff, rotate_rotate, UpwardEnumerable.le_iff_exists,
-      succMany?_rotate, rotate_inj]
-
-scoped instance :
-    LawfulUpwardEnumerable (BitVec n) where
-  ne_of_lt x y h := by
-    rw [← rotate_rotate (x := x), ← rotate_rotate (x := y)] at h ⊢
-    generalize rotate x = x at h ⊢
-    generalize rotate y = y at h ⊢
-    letI : UpwardEnumerable (BitVec n) := BitVec.instUpwardEnumerable
-    have : x ≠ y := by
-      apply UpwardEnumerable.ne_of_lt
-      obtain ⟨n, hn⟩ := h
-      refine ⟨n, ?_⟩
-      rwa [succMany?_rotate, rotate_map_eq_iff, Option.map_eq_map, Option.map_some, rotate_rotate] at hn
-    apply this.imp; intro heq
-    simpa [rotate_rotate] using congrArg rotate heq
-  succMany?_zero x := by
-    rw [← rotate_rotate (x := x)]
-    generalize rotate x = x
-    letI : UpwardEnumerable (BitVec n) := BitVec.instUpwardEnumerable
-    simp [succMany?_rotate, succMany?_zero]
-  succMany?_add_one m x := by
-    rw [← rotate_rotate (x := x)]
-    generalize rotate x = x
-    letI : UpwardEnumerable (BitVec n) := BitVec.instUpwardEnumerable
-    simp [succMany?_rotate, succMany?_add_one, Option.bind_map, Function.comp_def, succ?_rotate]
-
-scoped instance : LawfulUpwardEnumerableLT (BitVec n) := inferInstance
-scoped instance : LawfulUpwardEnumerableLT (BitVec n) := inferInstance
-
-scoped instance : Rxc.HasSize (BitVec n) where
-  size lo hi :=
-    haveI := BitVec.instHasSize (n := n)
-    Rxc.HasSize.size (rotate lo) (rotate hi)
-
-scoped instance : Rxc.LawfulHasSize (BitVec n) where
-  size_eq_zero_of_not_le bound x := by
-    simp only [LE.le]
-    match n with
-    | 0 => simp [eq_nil x, eq_nil bound]
-    | n + 1 =>
-      simp [BitVec.sle_iff_toInt_le, Rxc.HasSize.size,
-        toInt_eq_ofNat_toNat_rotate_sub (show n + 1 > 0 by omega)]
-      omega
-  size_eq_one_of_succ?_eq_none lo hi := by
-    rw [← rotate_rotate (x := lo)]
-    generalize rotate lo = lo
-    simp only [LE.le]
-    match n with
-    | 0 => simp [eq_nil lo, eq_nil hi, succ?, rotate, Rxc.HasSize.size, irredMin_def]
-    | n + 1 =>
-      simp [BitVec.sle_iff_toInt_le, toInt_eq_ofNat_toNat_rotate_sub,
-        Rxc.HasSize.size, rotate_rotate, succ?_rotate, Option.map_eq_map, Option.map_eq_none_iff,
-        succ?_eq_none]
-      omega
-  size_eq_succ_of_succ?_eq_some lo hi x := by
-    rw [← rotate_rotate (x := lo)]
-    generalize rotate lo = lo
-    simp only [LE.le]
-    match n with
-    | 0 => simp [eq_nil lo, eq_nil hi, succ?, rotate, Rxc.HasSize.size, irredMin_def]
-    | n + 1 =>
-      simp [BitVec.sle_iff_toInt_le, toInt_eq_ofNat_toNat_rotate_sub,
-        Rxc.HasSize.size, rotate_rotate, succ?_rotate, succ?_eq_some]
-      rintro h y h' hy rfl
-      simp only [rotate_rotate]
-      omega
-
-scoped instance : Rxc.IsAlwaysFinite (BitVec n) := inferInstance
-
-scoped instance : Rxo.HasSize (BitVec n) := .ofClosed
-scoped instance : Rxo.LawfulHasSize (BitVec n) := .of_closed
-scoped instance : Rxo.IsAlwaysFinite (BitVec n) := inferInstance
-
-scoped instance : Rxi.HasSize (BitVec n) where
-  size lo := 2 ^ n - (rotate lo).toNat
-
-scoped instance : Rxi.LawfulHasSize (BitVec n) where
-  size_eq_one_of_succ?_eq_none x := by
-    rw [← rotate_rotate (x := x)]
-    generalize rotate x = x
-    simp only [succ?_rotate, Option.map_eq_map, Option.map_eq_none_iff, Rxi.HasSize.size,
-      rotate_rotate]
-    letI := BitVec.instHasSize_2 (n := n)
-    exact Rxi.size_eq_one_of_succ?_eq_none x
-  size_eq_succ_of_succ?_eq_some lo lo' := by
-    rw [← rotate_rotate (x := lo), ← rotate_rotate (x := lo')]
-    generalize rotate lo = lo
-    generalize rotate lo' = lo'
-    simp [succ?_rotate, rotate_inj, instHasSize_2, rotate_rotate]
-    letI := BitVec.instHasSize_2 (n := n)
-    exact Rxi.size_eq_succ_of_succ?_eq_some lo lo'
-
-scoped instance : Rxi.IsAlwaysFinite (BitVec n) := inferInstance
-
-end Signed
-
+end
 end BitVec
