src/Init/Data/Range/Polymorphic/SInt.lean
@@ -11,11 +11,10 @@ public import Init.Data.Range.Polymorphic.Instances
 public import Init.Data.Order.Lemmas
 public import Init.Data.SInt
 import Init.Omega
-public import Init.Data.Range.Polymorphic.BitVec
 import Init.Data.Range.Polymorphic.UInt
 import all Init.Data.SInt.Basic
 
-public section
+import all Init.Data.Range.Polymorphic.Internal.SignedBitVec
 
 open Std Std.PRange
 
@@ -61,7 +60,8 @@ theorem succMany?_encode [m : HasModel α β] {x : α} :
 
 theorem eq_of_encode_eq [m : HasModel α β] (x y : α) :
     m.encode x = m.encode y → x = y := by
-  sorry
+  intro h
+  simpa [m.decode_encode] using congrArg m.decode h
 
 theorem encode_inj [m : HasModel α β] {x y : α} :
     m.encode x = m.encode y ↔ x = y := by
@@ -107,15 +107,6 @@ scoped instance instLawfulUpwardEnumerableLT [m : HasModel α β] :
 instance : Rxc.HasSize Int8 where
   size lo hi := (hi.toInt + 1 - lo.toInt).toNat
 
--- theorem rxcHasSize_eq_toBitVec :
---     Rxc.HasSize.size (Int8.ofBitVec lo) hi = Rxc.HasSize.size lo hi.toBitVec := by
---   simp [Rxc.HasSize.size, rotate, ← toInt_toBitVec, toInt_eq_ofNat_toNat_rotate_sub]
---   omega
-
--- private theorem ofBitVec_eq_iff {x : BitVec 8} {y : Int8} :
---     Int8.ofBitVec x = y ↔ x = y.toBitVec := by
---   rw [← toBitVec_ofBitVec x, toBitVec_inj, toBitVec_ofBitVec]
-
 scoped instance instRxcHasSize [m : HasModel α β] [Rxc.HasSize β] :
     Rxc.HasSize α where
   size lo hi := Rxc.HasSize.size (m.encode lo) (m.encode hi)
@@ -151,23 +142,27 @@ scoped instance instRxiLawfulHasSize [m : HasModel α β] [Rxi.HasSize β] [Rxi.
     simp only [this, instRxiHasSize]
     apply Rxi.LawfulHasSize.size_eq_succ_of_succ?_eq_some
 
-theorem general_succ? {α : Type u} [UpwardEnumerable α] [LE α] [LT α] [m : HasModel α (BitVec n)]
+private theorem general_succ? {α : Type u} [UpwardEnumerable α] [LE α] [LT α] [m : HasModel α (BitVec n)]
     {x : α}
-    (h : ∀ y, succ? x = some y ↔ ¬ m.encode x + 1#n = BitVec.Signed.irredMin n ∧ m.encode x + 1#n = m.encode y) :
+    (h : ∀ y, succ? x = some y ↔ ¬ m.encode x + 1#n = BitVec.Signed.intMinSealed n ∧ m.encode x + 1#n = m.encode y) :
     succ? x = (haveI := HasModel.instUpwardEnumerable (α := α); succ? x) := by
   ext y
   simp only [UpwardEnumerable.succ?, h]
   rw [← Option.map_inj_right HasModel.eq_of_encode_eq, Option.map_map, Function.comp_def]
   simp [HasModel.encode_decode, ← BitVec.eq_sub_iff_add_eq, rotate_eq_iff,
-    ← rotate_neg_eq_irredMin_sub, rotate_sub, rotate_rotate]
+    ← rotate_neg_eq_intMinSealed_sub, rotate_sub, rotate_rotate]
 
-theorem general_succMany? {α : Type u} [UpwardEnumerable α] [LE α] [LT α] [m : HasModel α (BitVec n)]
-    {x : α} {k} :
+private theorem general_succMany? {α : Type u} [UpwardEnumerable α] [LE α] [LT α]
+    [m : HasModel α (BitVec n)] {x : α} {k} :
     haveI := HasModel.instUpwardEnumerable (α := α)
-    succMany? k x = if (m.encode x).toInt + ↑k ≤ (BitVec.Signed.irredMax n).toInt then some (m.decode (BitVec.ofInt n ((m.encode x).toInt + ↑k))) else none := by
+    succMany? k x = if (m.encode x).toInt + ↑k ≤ (BitVec.Signed.intMaxSealed n).toInt then some (m.decode (BitVec.ofInt n ((m.encode x).toInt + ↑k))) else none := by
+  by_cases hn : n > 0; rotate_left
+  · cases show n = 0 by omega
+    simp [succMany?, BitVec.eq_nil (BitVec.Signed.rotate _), BitVec.eq_nil (.ofInt _ _),
+      BitVec.eq_nil (encode _), BitVec.eq_nil (BitVec.Signed.intMaxSealed _)]
   have h : ∀ a b c d : Int, a - b + c ≤ d - b ↔ a + c ≤ d := by omega
   simp [UpwardEnumerable.succMany?, BitVec.ofNatLT_eq_ofNat]
-  simp [toInt_eq_ofNat_toNat_rotate_sub' sorry, rotate_irredMax, h]
+  simp [toInt_eq_ofNat_toNat_rotate_sub' hn, rotate_intMaxSealed, h]
   simp only [← Int.natCast_add]
   congr
   · rw [Nat.lt_iff_add_one_le, Int.ofNat_le, Nat.le_sub_iff_add_le]
@@ -201,22 +196,23 @@ namespace Int8
 open BitVec.Signed
 open scoped HasModel
 
-@[inline] def irredMin := Int8.minValue
-@[inline] def irredMax := Int8.maxValue
-theorem irredMin_def : irredMin = Int8.minValue := (rfl)
-theorem irredMax_def : irredMax = Int8.maxValue := (rfl)
-seal irredMin irredMax
+@[inline] def minValueSealed := Int8.minValue
+@[inline] def maxValueSealed := Int8.maxValue
+theorem minValueSealed_def : minValueSealed = Int8.minValue := (rfl)
+theorem maxValueSealed_def : maxValueSealed = Int8.maxValue := (rfl)
+seal minValueSealed maxValueSealed
 
-theorem toBitVec_irredMin_eq_irredMin : irredMin.toBitVec = BitVec.Signed.irredMin 8 := by
-  simp [irredMin_def, BitVec.Signed.irredMin_def]
-theorem toBitVec_irredMax_eq_irredMax : irredMax.toBitVec = BitVec.Signed.irredMax 8 := by
-  simp [irredMax_def, BitVec.Signed.irredMax_def]
+theorem toBitVec_minValueSealed_eq_intMinSealed : minValueSealed.toBitVec = BitVec.Signed.intMinSealed 8 := by
+  simp [minValueSealed_def, BitVec.Signed.intMinSealed_def]
+theorem toBitVec_maxValueSealed_eq_intMaxSealed : maxValueSealed.toBitVec = BitVec.Signed.intMaxSealed 8 := by
+  simp [maxValueSealed_def, BitVec.Signed.intMaxSealed_def]
 
-instance : UpwardEnumerable Int8 where
-  succ? i := if i + 1 = irredMin then none else some (i + 1)
+@[no_expose]
+public instance : UpwardEnumerable Int8 where
+  succ? i := if i + 1 = minValueSealed then none else some (i + 1)
   succMany? n i :=
     have := i.minValue_le_toInt
-    if h : i.toInt + n ≤ irredMax.toInt then some (.ofIntLE _ (by omega) (irredMax_def ▸ h)) else none
+    if h : i.toInt + n ≤ maxValueSealed.toInt then some (.ofIntLE _ (by omega) (maxValueSealed_def ▸ h)) else none
 
 instance : HasModel Int8 (BitVec 8) where
   encode x := x.toBitVec
@@ -226,19 +222,15 @@ instance : HasModel Int8 (BitVec 8) where
   le_iff_encode_le := by simp [Int8.le_iff_toBitVec_sle, BitVec.Signed.instLE]
   lt_iff_encode_lt := by simp [Int8.lt_iff_toBitVec_slt, BitVec.Signed.instLT]
 
-private theorem ofBitVec_eq_iff {x : BitVec 8} {y : Int8} :
-    Int8.ofBitVec x = y ↔ x = y.toBitVec := by
-  rw [← toBitVec_ofBitVec x, toBitVec_inj, toBitVec_ofBitVec]
-
 theorem instUpwardEnumerable_eq :
     instUpwardEnumerable = HasModel.instUpwardEnumerable := by
   apply UpwardEnumerable.ext
   · apply funext; intro x
     apply HasModel.general_succ?
-    simp [HasModel.encode, succ?, ← Int8.toBitVec_inj, toBitVec_irredMin_eq_irredMin]
+    simp [HasModel.encode, succ?, ← Int8.toBitVec_inj, toBitVec_minValueSealed_eq_intMinSealed]
   · ext
     simp [HasModel.general_succMany?, instUpwardEnumerable, HasModel.encode, HasModel.decode,
-      ← toInt_toBitVec, toBitVec_irredMax_eq_irredMax, ofIntLE_eq_ofInt]
+      ← toInt_toBitVec, toBitVec_maxValueSealed_eq_intMaxSealed, ofIntLE_eq_ofInt]
 
 instance : LawfulUpwardEnumerable Int8 := by
   simp only [instUpwardEnumerable_eq]
@@ -248,27 +240,24 @@ instance : LawfulUpwardEnumerableLE Int8 := by
   simp only [instUpwardEnumerable_eq]
   infer_instance
 
-instance : LawfulUpwardEnumerableLT Int8 := inferInstance
-instance : LawfulUpwardEnumerableLT Int8 := inferInstance
-
-instance : Rxc.HasSize Int8 where
+public instance instRxcHasSize : Rxc.HasSize Int8 where
   size lo hi := (hi.toInt + 1 - lo.toInt).toNat
 
 theorem instRxcHasSize_eq :
-    instHasSize = HasModel.instRxcHasSize := by
-  simp only [instHasSize, HasModel.instRxcHasSize, Rxc.HasSize.size, HasModel.encode,
+    instRxcHasSize = HasModel.instRxcHasSize := by
+  simp only [instRxcHasSize, HasModel.instRxcHasSize, Rxc.HasSize.size, HasModel.encode,
     ← toInt_toBitVec, HasModel.general_rxcSize (Nat.zero_lt_succ _)]
 
-instance : Rxc.LawfulHasSize Int8 := by
+public instance instRxcLawfulHasSize : Rxc.LawfulHasSize Int8 := by
   simp only [instUpwardEnumerable_eq, instRxcHasSize_eq]
   infer_instance
-instance : Rxc.IsAlwaysFinite Int8 := inferInstance
+public instance : Rxc.IsAlwaysFinite Int8 := by exact inferInstance
 
-instance : Rxo.HasSize Int8 := .ofClosed
-instance : Rxo.LawfulHasSize Int8 := inferInstance
-instance : Rxo.IsAlwaysFinite Int8 := inferInstance
+public instance instRxoHasSize : Rxo.HasSize Int8 := .ofClosed
+public instance instRxoLawfulHasSize : Rxo.LawfulHasSize Int8 := by exact inferInstance
+public instance instRxoIsAlwaysFinite : Rxo.IsAlwaysFinite Int8 := by exact inferInstance
 
-instance instRxiHasSize : Rxi.HasSize Int8 where
+public instance instRxiHasSize : Rxi.HasSize Int8 where
   size lo := ((2 : Int) ^ 7 - lo.toInt).toNat
 
 theorem instRxiHasSize_eq :
@@ -276,10 +265,10 @@ theorem instRxiHasSize_eq :
   simp only [instRxiHasSize, HasModel.instRxiHasSize, Rxi.HasSize.size, ← toInt_toBitVec,
     HasModel.encode, HasModel.general_rxiSize (show 8 > 0 by omega)]
 
-instance : Rxi.LawfulHasSize Int8 := by
+public instance instRxiLawfulHasSize : Rxi.LawfulHasSize Int8 := by
   simp only [instUpwardEnumerable_eq, instRxiHasSize_eq]
   infer_instance
-instance : Rxi.IsAlwaysFinite Int8 := inferInstance
+public instance instRxiIsAlwaysFinite : Rxi.IsAlwaysFinite Int8 := by exact inferInstance
 
 end Int8
 
@@ -288,22 +277,23 @@ namespace Int16
 open BitVec.Signed
 open scoped HasModel
 
-@[inline] def irredMin := Int16.minValue
-@[inline] def irredMax := Int16.maxValue
-theorem irredMin_def : irredMin = Int16.minValue := (rfl)
-theorem irredMax_def : irredMax = Int16.maxValue := (rfl)
-seal irredMin irredMax
+@[inline] def minValueSealed := Int16.minValue
+@[inline] def maxValueSealed := Int16.maxValue
+theorem minValueSealed_def : minValueSealed = Int16.minValue := (rfl)
+theorem maxValueSealed_def : maxValueSealed = Int16.maxValue := (rfl)
+seal minValueSealed maxValueSealed
 
-theorem toBitVec_irredMin_eq_irredMin : irredMin.toBitVec = BitVec.Signed.irredMin 16 := by
-  simp [irredMin_def, BitVec.Signed.irredMin_def]
-theorem toBitVec_irredMax_eq_irredMax : irredMax.toBitVec = BitVec.Signed.irredMax 16 := by
-  simp [irredMax_def, BitVec.Signed.irredMax_def]
+theorem toBitVec_minValueSealed_eq_intMinSealed : minValueSealed.toBitVec = BitVec.Signed.intMinSealed 16 := by
+  simp [minValueSealed_def, BitVec.Signed.intMinSealed_def]
+theorem toBitVec_maxValueSealed_eq_intMaxSealed : maxValueSealed.toBitVec = BitVec.Signed.intMaxSealed 16 := by
+  simp [maxValueSealed_def, BitVec.Signed.intMaxSealed_def]
 
-instance : UpwardEnumerable Int16 where
-  succ? i := if i + 1 = irredMin then none else some (i + 1)
+@[no_expose]
+public instance : UpwardEnumerable Int16 where
+  succ? i := if i + 1 = minValueSealed then none else some (i + 1)
   succMany? n i :=
     have := i.minValue_le_toInt
-    if h : i.toInt + n ≤ irredMax.toInt then some (.ofIntLE _ (by omega) (irredMax_def ▸ h)) else none
+    if h : i.toInt + n ≤ maxValueSealed.toInt then some (.ofIntLE _ (by omega) (maxValueSealed_def ▸ h)) else none
 
 instance : HasModel Int16 (BitVec 16) where
   encode x := x.toBitVec
@@ -313,19 +303,15 @@ instance : HasModel Int16 (BitVec 16) where
   le_iff_encode_le := by simp [Int16.le_iff_toBitVec_sle, BitVec.Signed.instLE]
   lt_iff_encode_lt := by simp [Int16.lt_iff_toBitVec_slt, BitVec.Signed.instLT]
 
-private theorem ofBitVec_eq_iff {x : BitVec 16} {y : Int16} :
-    Int16.ofBitVec x = y ↔ x = y.toBitVec := by
-  rw [← toBitVec_ofBitVec x, toBitVec_inj, toBitVec_ofBitVec]
-
 theorem instUpwardEnumerable_eq :
     instUpwardEnumerable = HasModel.instUpwardEnumerable := by
   apply UpwardEnumerable.ext
   · apply funext; intro x
     apply HasModel.general_succ?
-    simp [HasModel.encode, succ?, ← Int16.toBitVec_inj, toBitVec_irredMin_eq_irredMin]
+    simp [HasModel.encode, succ?, ← Int16.toBitVec_inj, toBitVec_minValueSealed_eq_intMinSealed]
   · ext
     simp [HasModel.general_succMany?, instUpwardEnumerable, HasModel.encode, HasModel.decode,
-      ← toInt_toBitVec, toBitVec_irredMax_eq_irredMax, ofIntLE_eq_ofInt]
+      ← toInt_toBitVec, toBitVec_maxValueSealed_eq_intMaxSealed, ofIntLE_eq_ofInt]
 
 instance : LawfulUpwardEnumerable Int16 := by
   simp only [instUpwardEnumerable_eq]
@@ -335,27 +321,24 @@ instance : LawfulUpwardEnumerableLE Int16 := by
   simp only [instUpwardEnumerable_eq]
   infer_instance
 
-instance : LawfulUpwardEnumerableLT Int16 := inferInstance
-instance : LawfulUpwardEnumerableLT Int16 := inferInstance
-
-instance : Rxc.HasSize Int16 where
+public instance instRxcHasSize : Rxc.HasSize Int16 where
   size lo hi := (hi.toInt + 1 - lo.toInt).toNat
 
 theorem instRxcHasSize_eq :
-    instHasSize = HasModel.instRxcHasSize := by
-  simp only [instHasSize, HasModel.instRxcHasSize, Rxc.HasSize.size, HasModel.encode,
+    instRxcHasSize = HasModel.instRxcHasSize := by
+  simp only [instRxcHasSize, HasModel.instRxcHasSize, Rxc.HasSize.size, HasModel.encode,
     ← toInt_toBitVec, HasModel.general_rxcSize (Nat.zero_lt_succ _)]
 
-instance : Rxc.LawfulHasSize Int16 := by
+public instance instRxcLawfulHasSize : Rxc.LawfulHasSize Int16 := by
   simp only [instUpwardEnumerable_eq, instRxcHasSize_eq]
   infer_instance
-instance : Rxc.IsAlwaysFinite Int16 := inferInstance
+public instance : Rxc.IsAlwaysFinite Int16 := by exact inferInstance
 
-instance : Rxo.HasSize Int16 := .ofClosed
-instance : Rxo.LawfulHasSize Int16 := inferInstance
-instance : Rxo.IsAlwaysFinite Int16 := inferInstance
+public instance instRxoHasSize : Rxo.HasSize Int16 := .ofClosed
+public instance instRxoLawfulHasSize : Rxo.LawfulHasSize Int16 := by exact inferInstance
+public instance instRxoIsAlwaysFinite : Rxo.IsAlwaysFinite Int16 := by exact inferInstance
 
-instance instRxiHasSize : Rxi.HasSize Int16 where
+public instance instRxiHasSize : Rxi.HasSize Int16 where
   size lo := ((2 : Int) ^ 15 - lo.toInt).toNat
 
 theorem instRxiHasSize_eq :
@@ -363,10 +346,10 @@ theorem instRxiHasSize_eq :
   simp only [instRxiHasSize, HasModel.instRxiHasSize, Rxi.HasSize.size, ← toInt_toBitVec,
     HasModel.encode, HasModel.general_rxiSize (show 16 > 0 by omega)]
 
-instance : Rxi.LawfulHasSize Int16 := by
+public instance instRxiLawfulHasSize : Rxi.LawfulHasSize Int16 := by
   simp only [instUpwardEnumerable_eq, instRxiHasSize_eq]
   infer_instance
-instance : Rxi.IsAlwaysFinite Int16 := inferInstance
+public instance instRxiIsAlwaysFinite : Rxi.IsAlwaysFinite Int16 := by exact inferInstance
 
 end Int16
 
@@ -375,22 +358,23 @@ namespace Int32
 open BitVec.Signed
 open scoped HasModel
 
-@[inline] def irredMin := Int32.minValue
-@[inline] def irredMax := Int32.maxValue
-theorem irredMin_def : irredMin = Int32.minValue := (rfl)
-theorem irredMax_def : irredMax = Int32.maxValue := (rfl)
-seal irredMin irredMax
+@[inline] def minValueSealed := Int32.minValue
+@[inline] def maxValueSealed := Int32.maxValue
+theorem minValueSealed_def : minValueSealed = Int32.minValue := (rfl)
+theorem maxValueSealed_def : maxValueSealed = Int32.maxValue := (rfl)
+seal minValueSealed maxValueSealed
 
-theorem toBitVec_irredMin_eq_irredMin : irredMin.toBitVec = BitVec.Signed.irredMin 32 := by
-  simp [irredMin_def, BitVec.Signed.irredMin_def]
-theorem toBitVec_irredMax_eq_irredMax : irredMax.toBitVec = BitVec.Signed.irredMax 32 := by
-  simp [irredMax_def, BitVec.Signed.irredMax_def]
+theorem toBitVec_minValueSealed_eq_intMinSealed : minValueSealed.toBitVec = BitVec.Signed.intMinSealed 32 := by
+  simp [minValueSealed_def, BitVec.Signed.intMinSealed_def]
+theorem toBitVec_maxValueSealed_eq_intMaxSealed : maxValueSealed.toBitVec = BitVec.Signed.intMaxSealed 32 := by
+  simp [maxValueSealed_def, BitVec.Signed.intMaxSealed_def]
 
-instance : UpwardEnumerable Int32 where
-  succ? i := if i + 1 = irredMin then none else some (i + 1)
+@[no_expose]
+public instance : UpwardEnumerable Int32 where
+  succ? i := if i + 1 = minValueSealed then none else some (i + 1)
   succMany? n i :=
     have := i.minValue_le_toInt
-    if h : i.toInt + n ≤ irredMax.toInt then some (.ofIntLE _ (by omega) (irredMax_def ▸ h)) else none
+    if h : i.toInt + n ≤ maxValueSealed.toInt then some (.ofIntLE _ (by omega) (maxValueSealed_def ▸ h)) else none
 
 instance : HasModel Int32 (BitVec 32) where
   encode x := x.toBitVec
@@ -400,19 +384,15 @@ instance : HasModel Int32 (BitVec 32) where
   le_iff_encode_le := by simp [Int32.le_iff_toBitVec_sle, BitVec.Signed.instLE]
   lt_iff_encode_lt := by simp [Int32.lt_iff_toBitVec_slt, BitVec.Signed.instLT]
 
-private theorem ofBitVec_eq_iff {x : BitVec 32} {y : Int32} :
-    Int32.ofBitVec x = y ↔ x = y.toBitVec := by
-  rw [← toBitVec_ofBitVec x, toBitVec_inj, toBitVec_ofBitVec]
-
 theorem instUpwardEnumerable_eq :
     instUpwardEnumerable = HasModel.instUpwardEnumerable := by
   apply UpwardEnumerable.ext
   · apply funext; intro x
     apply HasModel.general_succ?
-    simp [HasModel.encode, succ?, ← Int32.toBitVec_inj, toBitVec_irredMin_eq_irredMin]
+    simp [HasModel.encode, succ?, ← Int32.toBitVec_inj, toBitVec_minValueSealed_eq_intMinSealed]
   · ext
     simp [HasModel.general_succMany?, instUpwardEnumerable, HasModel.encode, HasModel.decode,
-      ← toInt_toBitVec, toBitVec_irredMax_eq_irredMax, ofIntLE_eq_ofInt]
+      ← toInt_toBitVec, toBitVec_maxValueSealed_eq_intMaxSealed, ofIntLE_eq_ofInt]
 
 instance : LawfulUpwardEnumerable Int32 := by
   simp only [instUpwardEnumerable_eq]
@@ -422,27 +402,24 @@ instance : LawfulUpwardEnumerableLE Int32 := by
   simp only [instUpwardEnumerable_eq]
   infer_instance
 
-instance : LawfulUpwardEnumerableLT Int32 := inferInstance
-instance : LawfulUpwardEnumerableLT Int32 := inferInstance
-
-instance : Rxc.HasSize Int32 where
+public instance instRxcHasSize : Rxc.HasSize Int32 where
   size lo hi := (hi.toInt + 1 - lo.toInt).toNat
 
 theorem instRxcHasSize_eq :
-    instHasSize = HasModel.instRxcHasSize := by
-  simp only [instHasSize, HasModel.instRxcHasSize, Rxc.HasSize.size, HasModel.encode,
+    instRxcHasSize = HasModel.instRxcHasSize := by
+  simp only [instRxcHasSize, HasModel.instRxcHasSize, Rxc.HasSize.size, HasModel.encode,
     ← toInt_toBitVec, HasModel.general_rxcSize (Nat.zero_lt_succ _)]
 
-instance : Rxc.LawfulHasSize Int32 := by
+public instance instRxcLawfulHasSize : Rxc.LawfulHasSize Int32 := by
   simp only [instUpwardEnumerable_eq, instRxcHasSize_eq]
   infer_instance
-instance : Rxc.IsAlwaysFinite Int32 := inferInstance
+public instance : Rxc.IsAlwaysFinite Int32 := by exact inferInstance
 
-instance : Rxo.HasSize Int32 := .ofClosed
-instance : Rxo.LawfulHasSize Int32 := inferInstance
-instance : Rxo.IsAlwaysFinite Int32 := inferInstance
+public instance instRxoHasSize : Rxo.HasSize Int32 := .ofClosed
+public instance instRxoLawfulHasSize : Rxo.LawfulHasSize Int32 := by exact inferInstance
+public instance instRxoIsAlwaysFinite : Rxo.IsAlwaysFinite Int32 := by exact inferInstance
 
-instance instRxiHasSize : Rxi.HasSize Int32 where
+public instance instRxiHasSize : Rxi.HasSize Int32 where
   size lo := ((2 : Int) ^ 31 - lo.toInt).toNat
 
 theorem instRxiHasSize_eq :
@@ -450,10 +427,10 @@ theorem instRxiHasSize_eq :
   simp only [instRxiHasSize, HasModel.instRxiHasSize, Rxi.HasSize.size, ← toInt_toBitVec,
     HasModel.encode, HasModel.general_rxiSize (show 32 > 0 by omega)]
 
-instance : Rxi.LawfulHasSize Int32 := by
+public instance instRxiLawfulHasSize : Rxi.LawfulHasSize Int32 := by
   simp only [instUpwardEnumerable_eq, instRxiHasSize_eq]
   infer_instance
-instance : Rxi.IsAlwaysFinite Int32 := inferInstance
+public instance instRxiIsAlwaysFinite : Rxi.IsAlwaysFinite Int32 := by exact inferInstance
 
 end Int32
 
@@ -462,22 +439,23 @@ namespace Int64
 open BitVec.Signed
 open scoped HasModel
 
-@[inline] def irredMin := Int64.minValue
-@[inline] def irredMax := Int64.maxValue
-theorem irredMin_def : irredMin = Int64.minValue := (rfl)
-theorem irredMax_def : irredMax = Int64.maxValue := (rfl)
-seal irredMin irredMax
+@[inline] def minValueSealed := Int64.minValue
+@[inline] def maxValueSealed := Int64.maxValue
+theorem minValueSealed_def : minValueSealed = Int64.minValue := (rfl)
+theorem maxValueSealed_def : maxValueSealed = Int64.maxValue := (rfl)
+seal minValueSealed maxValueSealed
 
-theorem toBitVec_irredMin_eq_irredMin : irredMin.toBitVec = BitVec.Signed.irredMin 64 := by
-  simp [irredMin_def, BitVec.Signed.irredMin_def]
-theorem toBitVec_irredMax_eq_irredMax : irredMax.toBitVec = BitVec.Signed.irredMax 64 := by
-  simp [irredMax_def, BitVec.Signed.irredMax_def]
+theorem toBitVec_minValueSealed_eq_intMinSealed : minValueSealed.toBitVec = BitVec.Signed.intMinSealed 64 := by
+  simp [minValueSealed_def, BitVec.Signed.intMinSealed_def]
+theorem toBitVec_maxValueSealed_eq_intMaxSealed : maxValueSealed.toBitVec = BitVec.Signed.intMaxSealed 64 := by
+  simp [maxValueSealed_def, BitVec.Signed.intMaxSealed_def]
 
-instance : UpwardEnumerable Int64 where
-  succ? i := if i + 1 = irredMin then none else some (i + 1)
+@[no_expose]
+public instance : UpwardEnumerable Int64 where
+  succ? i := if i + 1 = minValueSealed then none else some (i + 1)
   succMany? n i :=
     have := i.minValue_le_toInt
-    if h : i.toInt + n ≤ irredMax.toInt then some (.ofIntLE _ (by omega) (irredMax_def ▸ h)) else none
+    if h : i.toInt + n ≤ maxValueSealed.toInt then some (.ofIntLE _ (by omega) (maxValueSealed_def ▸ h)) else none
 
 instance : HasModel Int64 (BitVec 64) where
   encode x := x.toBitVec
@@ -487,19 +465,15 @@ instance : HasModel Int64 (BitVec 64) where
   le_iff_encode_le := by simp [Int64.le_iff_toBitVec_sle, BitVec.Signed.instLE]
   lt_iff_encode_lt := by simp [Int64.lt_iff_toBitVec_slt, BitVec.Signed.instLT]
 
-private theorem ofBitVec_eq_iff {x : BitVec 64} {y : Int64} :
-    Int64.ofBitVec x = y ↔ x = y.toBitVec := by
-  rw [← toBitVec_ofBitVec x, toBitVec_inj, toBitVec_ofBitVec]
-
 theorem instUpwardEnumerable_eq :
     instUpwardEnumerable = HasModel.instUpwardEnumerable := by
   apply UpwardEnumerable.ext
   · apply funext; intro x
     apply HasModel.general_succ?
-    simp [HasModel.encode, succ?, ← Int64.toBitVec_inj, toBitVec_irredMin_eq_irredMin]
+    simp [HasModel.encode, succ?, ← Int64.toBitVec_inj, toBitVec_minValueSealed_eq_intMinSealed]
   · ext
     simp [HasModel.general_succMany?, instUpwardEnumerable, HasModel.encode, HasModel.decode,
-      ← toInt_toBitVec, toBitVec_irredMax_eq_irredMax, ofIntLE_eq_ofInt]
+      ← toInt_toBitVec, toBitVec_maxValueSealed_eq_intMaxSealed, ofIntLE_eq_ofInt]
 
 instance : LawfulUpwardEnumerable Int64 := by
   simp only [instUpwardEnumerable_eq]
@@ -509,27 +483,24 @@ instance : LawfulUpwardEnumerableLE Int64 := by
   simp only [instUpwardEnumerable_eq]
   infer_instance
 
-instance : LawfulUpwardEnumerableLT Int64 := inferInstance
-instance : LawfulUpwardEnumerableLT Int64 := inferInstance
-
-instance : Rxc.HasSize Int64 where
+public instance instRxcHasSize : Rxc.HasSize Int64 where
   size lo hi := (hi.toInt + 1 - lo.toInt).toNat
 
 theorem instRxcHasSize_eq :
-    instHasSize = HasModel.instRxcHasSize := by
-  simp only [instHasSize, HasModel.instRxcHasSize, Rxc.HasSize.size, HasModel.encode,
+    instRxcHasSize = HasModel.instRxcHasSize := by
+  simp only [instRxcHasSize, HasModel.instRxcHasSize, Rxc.HasSize.size, HasModel.encode,
     ← toInt_toBitVec, HasModel.general_rxcSize (Nat.zero_lt_succ _)]
 
-instance : Rxc.LawfulHasSize Int64 := by
+public instance instRxcLawfulHasSize : Rxc.LawfulHasSize Int64 := by
   simp only [instUpwardEnumerable_eq, instRxcHasSize_eq]
   infer_instance
-instance : Rxc.IsAlwaysFinite Int64 := inferInstance
+public instance : Rxc.IsAlwaysFinite Int64 := by exact inferInstance
 
-instance : Rxo.HasSize Int64 := .ofClosed
-instance : Rxo.LawfulHasSize Int64 := inferInstance
-instance : Rxo.IsAlwaysFinite Int64 := inferInstance
+public instance instRxoHasSize : Rxo.HasSize Int64 := .ofClosed
+public instance instRxoLawfulHasSize : Rxo.LawfulHasSize Int64 := by exact inferInstance
+public instance instRxoIsAlwaysFinite : Rxo.IsAlwaysFinite Int64 := by exact inferInstance
 
-instance instRxiHasSize : Rxi.HasSize Int64 where
+public instance instRxiHasSize : Rxi.HasSize Int64 where
   size lo := ((2 : Int) ^ 63 - lo.toInt).toNat
 
 theorem instRxiHasSize_eq :
@@ -537,10 +508,10 @@ theorem instRxiHasSize_eq :
   simp only [instRxiHasSize, HasModel.instRxiHasSize, Rxi.HasSize.size, ← toInt_toBitVec,
     HasModel.encode, HasModel.general_rxiSize (show 64 > 0 by omega)]
 
-instance : Rxi.LawfulHasSize Int64 := by
+public instance instRxiLawfulHasSize : Rxi.LawfulHasSize Int64 := by
   simp only [instUpwardEnumerable_eq, instRxiHasSize_eq]
   infer_instance
-instance : Rxi.IsAlwaysFinite Int64 := inferInstance
+public instance instRxiIsAlwaysFinite : Rxi.IsAlwaysFinite Int64 := by exact inferInstance
 
 end Int64
 
@@ -549,28 +520,29 @@ namespace ISize
 open BitVec.Signed
 open scoped HasModel
 
-@[inline] def irredMin := ISize.minValue
-@[inline] def irredMax := ISize.maxValue
-theorem irredMin_def : irredMin = ISize.minValue := (rfl)
-theorem irredMax_def : irredMax = ISize.maxValue := (rfl)
-seal irredMin irredMax
+@[inline] def minValueSealed := ISize.minValue
+@[inline] def maxValueSealed := ISize.maxValue
+theorem minValueSealed_def : minValueSealed = ISize.minValue := (rfl)
+theorem maxValueSealed_def : maxValueSealed = ISize.maxValue := (rfl)
+seal minValueSealed maxValueSealed
 
-theorem toBitVec_irredMin_eq_irredMin :
-    irredMin.toBitVec = BitVec.Signed.irredMin System.Platform.numBits := by
-  rw [irredMin_def, BitVec.Signed.irredMin_def, toBitVec_minValue]
+private theorem toBitVec_minValueSealed_eq_intMinSealed :
+    minValueSealed.toBitVec = BitVec.Signed.intMinSealed System.Platform.numBits := by
+  rw [minValueSealed_def, BitVec.Signed.intMinSealed_def, toBitVec_minValue]
   have := System.Platform.numBits_eq; generalize System.Platform.numBits = a at this ⊢
   rcases this with rfl | rfl <;> rfl
-theorem toBitVec_irredMax_eq_irredMax :
-    irredMax.toBitVec = BitVec.Signed.irredMax System.Platform.numBits := by
-  rw [irredMax_def, BitVec.Signed.irredMax_def, toBitVec_maxValue]
+private theorem toBitVec_maxValueSealed_eq_intMaxSealed :
+    maxValueSealed.toBitVec = BitVec.Signed.intMaxSealed System.Platform.numBits := by
+  rw [maxValueSealed_def, BitVec.Signed.intMaxSealed_def, toBitVec_maxValue]
   have := System.Platform.numBits_eq; generalize System.Platform.numBits = a at this ⊢
   rcases this with rfl | rfl <;> rfl
 
-instance : UpwardEnumerable ISize where
-  succ? i := if i + 1 = irredMin then none else some (i + 1)
+@[no_expose]
+public instance : UpwardEnumerable ISize where
+  succ? i := if i + 1 = minValueSealed then none else some (i + 1)
   succMany? n i :=
     have := i.minValue_le_toInt
-    if h : i.toInt + n ≤ irredMax.toInt then some (.ofIntLE _ (by omega) (irredMax_def ▸ h)) else none
+    if h : i.toInt + n ≤ maxValueSealed.toInt then some (.ofIntLE _ (by omega) (maxValueSealed_def ▸ h)) else none
 
 instance : HasModel ISize (BitVec System.Platform.numBits) where
   encode x := x.toBitVec
@@ -580,19 +552,15 @@ instance : HasModel ISize (BitVec System.Platform.numBits) where
   le_iff_encode_le := by simp [ISize.le_iff_toBitVec_sle, BitVec.Signed.instLE]
   lt_iff_encode_lt := by simp [ISize.lt_iff_toBitVec_slt, BitVec.Signed.instLT]
 
-private theorem ofBitVec_eq_iff {x : BitVec System.Platform.numBits} {y : ISize} :
-    ISize.ofBitVec x = y ↔ x = y.toBitVec := by
-  rw [← toBitVec_ofBitVec x, toBitVec_inj, toBitVec_ofBitVec]
-
 theorem instUpwardEnumerable_eq :
     instUpwardEnumerable = HasModel.instUpwardEnumerable := by
   apply UpwardEnumerable.ext
   · apply funext; intro x
     apply HasModel.general_succ?
-    simp [HasModel.encode, succ?, ← ISize.toBitVec_inj, toBitVec_irredMin_eq_irredMin]
+    simp [HasModel.encode, succ?, ← ISize.toBitVec_inj, toBitVec_minValueSealed_eq_intMinSealed]
   · ext
     simp [HasModel.general_succMany?, instUpwardEnumerable, HasModel.encode, HasModel.decode,
-      ← toInt_toBitVec, toBitVec_irredMax_eq_irredMax, ofIntLE_eq_ofInt]
+      ← toInt_toBitVec, toBitVec_maxValueSealed_eq_intMaxSealed, ofIntLE_eq_ofInt]
 
 instance : LawfulUpwardEnumerable ISize := by
   simp only [instUpwardEnumerable_eq]
@@ -602,27 +570,24 @@ instance : LawfulUpwardEnumerableLE ISize := by
   simp only [instUpwardEnumerable_eq]
   infer_instance
 
-instance : LawfulUpwardEnumerableLT ISize := inferInstance
-instance : LawfulUpwardEnumerableLT ISize := inferInstance
-
-instance : Rxc.HasSize ISize where
+public instance instRxcHasSize : Rxc.HasSize ISize where
   size lo hi := (hi.toInt + 1 - lo.toInt).toNat
 
 theorem instRxcHasSize_eq :
-    instHasSize = HasModel.instRxcHasSize := by
-  simp only [instHasSize, HasModel.instRxcHasSize, Rxc.HasSize.size, HasModel.encode,
+    instRxcHasSize = HasModel.instRxcHasSize := by
+  simp only [instRxcHasSize, HasModel.instRxcHasSize, Rxc.HasSize.size, HasModel.encode,
     ← toInt_toBitVec, HasModel.general_rxcSize System.Platform.numBits_pos]
 
-instance : Rxc.LawfulHasSize ISize := by
+public instance instRxcLawfulHasSize : Rxc.LawfulHasSize ISize := by
   simp only [instUpwardEnumerable_eq, instRxcHasSize_eq]
   infer_instance
-instance : Rxc.IsAlwaysFinite ISize := inferInstance
+public instance : Rxc.IsAlwaysFinite ISize := by exact inferInstance
 
-instance : Rxo.HasSize ISize := .ofClosed
-instance : Rxo.LawfulHasSize ISize := inferInstance
-instance : Rxo.IsAlwaysFinite ISize := inferInstance
+public instance instRxoHasSize : Rxo.HasSize ISize := .ofClosed
+public instance instRxoLawfulHasSize : Rxo.LawfulHasSize ISize := by exact inferInstance
+public instance instRxoIsAlwaysFinite : Rxo.IsAlwaysFinite ISize := by exact inferInstance
 
-instance instRxiHasSize : Rxi.HasSize ISize where
+public instance instRxiHasSize : Rxi.HasSize ISize where
   size lo := ((2 : Int) ^ (System.Platform.numBits - 1) - lo.toInt).toNat
 
 theorem instRxiHasSize_eq :
@@ -630,9 +595,9 @@ theorem instRxiHasSize_eq :
   simp only [instRxiHasSize, HasModel.instRxiHasSize, Rxi.HasSize.size, ← toInt_toBitVec,
     HasModel.encode, HasModel.general_rxiSize System.Platform.numBits_pos]
 
-instance : Rxi.LawfulHasSize ISize := by
+public instance instRxiLawfulHasSize : Rxi.LawfulHasSize ISize := by
   simp only [instUpwardEnumerable_eq, instRxiHasSize_eq]
   infer_instance
-instance : Rxi.IsAlwaysFinite ISize := inferInstance
+public instance instRxiIsAlwaysFinite : Rxi.IsAlwaysFinite ISize := by exact inferInstance
 
 end ISize
